Finally got around to fleshing out the real simpset (the other changes are the ramifications of this!)
Major changes:

1. Got rid of AC rewrites for + and *. If you want them (perhaps for
compatibility with the old real_ss), use real_ac_ss.

2. Added a huge bunch of useful rewrites to real_ss, though I'm sure
I'll need to add a huge bunch more before I'm finished with it.

src/real/realSimps.sig
@@ -1,6 +1,16 @@
 signature realSimps =
 sig
-   val real_ss : simpLib.simpset
 
-   (* Incorporates simpsets for bool, pair, and arithmetic *)
+  (* Useful rewrites for basic real arithmetic *)
+  val real_SS : simpLib.ssdata
+    
+  (* Incorporates simpsets for bool, pair, and arithmetic *)
+  val real_ss : simpLib.simpset
+    
+  (* AC rewrites for + and *: occasionally useful *)
+  val real_ac_SS : simpLib.ssdata
+    
+  (* Incorporates the real simpset *)
+  val real_ac_ss : simpLib.simpset
+
 end
