src/real/realSimps.sml
@@ -1,6 +1,5 @@
 (* ------------------------------------------------------------------------- *)
-(* A real simpset (includes Peano arithmetic and pairs).  This should be     *)
-(* fleshed out.                                                              *)
+(* A real simpset (includes Peano arithmetic and pairs).                     *)
 (* ------------------------------------------------------------------------- *)
 
 structure realSimps :> realSimps = 
@@ -12,15 +11,34 @@ val arith_ss =
   simpLib.++
     (simpLib.++(boolSimps.bool_ss, pairSimps.PAIR_ss),numSimps.ARITH_ss);
 
+val real_SS = simpLib.SIMPSET
+  {ac = [],
+   congs = [],
+   convs = [],
+   dprocs = [],
+   filter = NONE,
+   rewrs = [REAL_ADD_LID, REAL_ADD_RID, REAL_MUL_LID, REAL_MUL_RID, 
+            REAL_MUL_LZERO, REAL_MUL_RZERO,
+            REAL_LE_REFL, REAL_SUB_REFL, REAL_SUB_RZERO, REAL_LE_01,
+            REAL_SUB_ADD2, REAL_MUL_SUB2_CANCEL, REAL_NEG_HALF,
+            REAL_LE_SUB_CANCEL2, REAL_LT_HALF1, REAL_HALF_BETWEEN, REAL_LT_01,
+            REAL_MUL_SUB1_CANCEL, REAL_NEG_THIRD, REAL_DIV2_CANCEL2,
+            REAL_DIV3_CANCEL2, REAL_OVER1, REAL_THIRDS_BETWEEN,
+            REAL_DIV_ADD, REAL_DIV2_MUL_CANCEL, REAL_DIV3_MUL_CANCEL, REAL_INJ,
+            REAL_ADD, REAL_LE, REAL_LT, REAL_MUL, REAL_LT_INV_EQ,
+            REAL_POS_POS, REAL_POS_INFLATE, REAL_MIN_REFL, REAL_MIN_LE]};
 
-val real_ss = simpLib.++(arith_ss, simpLib.SIMPSET {
+val real_ss = simpLib.++ (arith_ss, real_SS);
+
+val real_ac_SS = simpLib.SIMPSET {
   ac = [(SPEC_ALL REAL_ADD_ASSOC, SPEC_ALL REAL_ADD_SYM),
         (SPEC_ALL REAL_MUL_ASSOC, SPEC_ALL REAL_MUL_SYM)],
   convs = [],
   dprocs = [],
   filter = NONE,
-  rewrs = [REAL_ADD_LID, REAL_ADD_RID, REAL_MUL_LID, REAL_MUL_RID, 
-           REAL_MUL_LZERO, REAL_MUL_RZERO],
-  congs = []});
+  rewrs = [],
+  congs = []};
+
+val real_ac_ss = simpLib.++ (real_ss, real_ac_SS);
 
 end;
